theories/heap_lang/tactics.v
@@ -210,7 +210,7 @@ Ltac solve_closed :=
 Hint Extern 0 (Closed _ _) => solve_closed : typeclass_instances.
 
 Ltac solve_to_val :=
-  rewrite /IntoVal;
+  rewrite /AsVal /IntoVal;
   try match goal with
   | |- context E [language.to_val ?e] =>
      let X := context E [to_val e] in change X
@@ -224,6 +224,7 @@ Ltac solve_to_val :=
      apply W.to_val_is_Some, (bool_decide_unpack _); vm_compute; exact I
   end.
 Hint Extern 10 (IntoVal _ _) => solve_to_val : typeclass_instances.
+Hint Extern 10 (AsVal _) => solve_to_val : typeclass_instances.
 
 Ltac solve_atomic :=
   match goal with
